definitions/typing.v
@@ -8,55 +8,131 @@ Open Scope system_t_term_scope.
 
 Module FMap := FIdent.Map.
 
-Record context := {
-  bmap : list typeT;
-  fmap : FMap.t typeT
-}.
+Module FMapFacts := Coq.FSets.FMapFacts.WFacts FMap.
 
-Definition bpush (t : typeT) (G : context) := {|
-  bmap := t :: (bmap G);
-  fmap := fmap G
-|}.
+Module Context.
 
-Inductive typing_derivation : context -> termT -> typeT -> Type :=
+  Record t := {
+    bmap : list typeT;
+    fmap : FMap.t typeT
+  }.
+
+  Definition empty : t := {|
+    bmap := List.nil;
+    fmap := FMap.empty typeT
+  |}.
+
+  Definition map (f : typeT -> typeT) (G : t) := {|
+    bmap := List.map f (bmap G);
+    fmap := FMap.map f (fmap G)
+  |}.
+
+  Definition context_par_tsubst (s : TMap.t typeT) : t -> t :=
+    map (typeT_par_tsubst s).
+
+  Definition bpush (u : typeT) (G : t) := {|
+    bmap := u :: (bmap G);
+    fmap := fmap G
+  |}.
+
+  Definition Equal (G H : t) :=
+    (bmap G) = (bmap H) /\ FMap.Equal (fmap G) (fmap H).
+  
+  #[export] Instance equivalence : Equivalence Equal.
+  Proof.
+    constructor; constructor; auto using FMapFacts.Equal_refl.
+    - destruct H as [H _].
+      rewrite H.
+      reflexivity.
+    - destruct H as [_ H].
+      apply FMapFacts.Equal_sym.
+      exact H.
+    - destruct H as [H _].
+      destruct H0 as [I _].
+      rewrite H.
+      rewrite I.
+      reflexivity.
+    - destruct H as [_ H].
+      destruct H0 as [_ I].
+      eapply FMapFacts.Equal_trans.
+    --- exact H.
+    --- exact I.
+  Qed.
+
+  Notation " x == y " := (Equal x y) (at level 70, no associativity).
+
+  Notation " x =/= y " := (complement Equal x y) (at level 70, no associativity).
+
+End Context.
+
+Inductive derivation : Context.t -> termT -> typeT -> Prop :=
   | bvarT_ax :
-    forall G : context, forall n : nat, forall t : typeT,
-    nth_error (bmap G) n = Some t ->
-    typing_derivation G (bvarT n) t
+    forall G : Context.t, forall n : nat, forall t : typeT,
+    nth_error (Context.bmap G) n = Some t ->
+    derivation G (bvarT n) t
   | fvarT_ax :
-    forall G : context, forall x : fident, forall t : typeT,
-    FMap.MapsTo x t (fmap G) ->
-    typing_derivation G (fvarT x) t
+    forall G : Context.t, forall x : fident, forall t : typeT,
+    FMap.MapsTo x t (Context.fmap G) ->
+    derivation G (fvarT x) t
   | absT_in :
-    forall G : context, forall e : termT, forall t u : typeT,
-    typing_derivation (bpush t G) e u ->
-    typing_derivation G (absT e) (t ->T u)
+    forall G : Context.t, forall e : termT, forall t u : typeT,
+    derivation (Context.bpush t G) e u ->
+    derivation G (absT e) (t ->T u)
   | appT_el :
-    forall G : context, forall e f : termT, forall t u : typeT,
-    typing_derivation G e (t ->T u) ->
-    typing_derivation G f t ->
-    typing_derivation G (appT e f) u
+    forall G : Context.t, forall e f : termT, forall t u : typeT,
+    derivation G e (t ->T u) ->
+    derivation G f t ->
+    derivation G (appT e f) u
   | trueT_ax :
-    forall G : context, typing_derivation G trueT boolT
+    forall G : Context.t, derivation G trueT boolT
   | falseT_ax :
-    forall G : context, typing_derivation G falseT boolT
+    forall G : Context.t, derivation G falseT boolT
   | iteT_el :
-    forall G : context, forall e f g : termT, forall t : typeT,
-    typing_derivation G e boolT ->
-    typing_derivation G f t ->
-    typing_derivation G g t ->
-    typing_derivation G (iteT e f g) t
+    forall G : Context.t, forall e f g : termT, forall t : typeT,
+    derivation G e boolT ->
+    derivation G f t ->
+    derivation G g t ->
+    derivation G (iteT e f g) t
   | oT_ax :
-    forall G : context, typing_derivation G oT natT
+    forall G : Context.t, derivation G oT natT
   | sT_el :
-    forall G : context, forall e : termT, typing_derivation G e natT ->
-    typing_derivation G (sT e) natT
+    forall G : Context.t, forall e : termT,
+    derivation G e natT ->
+    derivation G (sT e) natT
   | recT_el :
-    forall G : context, forall e f g : termT, forall t : typeT,
-    typing_derivation G e t ->
-    typing_derivation G f (t ->T natT ->T t) ->
-    typing_derivation G g natT ->
-    typing_derivation G (recT e f g) t.
+    forall G : Context.t, forall e f g : termT, forall t : typeT,
+    derivation G e t ->
+    derivation G f (t ->T natT ->T t) ->
+    derivation G g natT ->
+    derivation G (recT e f g) t.
+
+(** Given a type substitution and a typing derivation, applying
+    that substitution to the context and all types appearing in the
+    derivation yields a new derivation.
+*)
+Lemma derivation_par_tsubst
+  {G : Context.t} {e : termT} {t : typeT}
+  (s : TMap.t typeT) (D : derivation G e t) :
+  derivation (Context.context_par_tsubst s G) e (typeT_par_tsubst s t).
+Proof.
+  induction D;
+  eauto using derivation;
+  simpl.
+  - apply bvarT_ax.
+    simpl.
+    apply List.map_nth_error.
+    exact H.
+  - apply fvarT_ax.
+    simpl.
+    apply FMap.map_1.
+    exact H.
+Qed.
+
+Lemma typing_id (t : typeT) :
+    derivation Context.empty (absT (bvarT O)) (t ->T t).
+Proof.
+  eauto using derivation.
+Qed.
 
 Close Scope system_t_type_scope.
 Close Scope system_t_term_scope.
